Put main search execution and soundness and completeness proofs to searchcommon

Graphlib/SearchAlgorithm.lean
@@ -291,3 +291,204 @@ lemma search_recurse_lift_base_invariant
       constructor
       · use invar_holds_on_base
       · use invar_carries
+
+
+def search_internal {state_type : Type} [has_base_search_state g state_type]
+    (start : V)
+    (goal : V)
+    (start_to_state : V → state_type)
+    (search_step : search_step_function g)
+    (termination_metric : state_type → ℕ × ℕ)
+    (decreasing_proof : termination_metric_decreasing_proof goal search_step termination_metric):
+    state_type × Bool :=
+  search_recurse goal (start_to_state start) search_step termination_metric decreasing_proof
+
+
+
+abbrev search_visited_goal_if_returned_true {state_type : Type} [has_base_search_state g state_type]
+    (start : V)
+    (goal : V)
+    (start_to_state : V → state_type)
+    (search_step : search_step_function g)
+    (termination_metric : state_type → ℕ × ℕ)
+    (decreasing_proof : termination_metric_decreasing_proof goal search_step termination_metric):=
+    let ret := (search_internal start goal start_to_state search_step termination_metric decreasing_proof)
+    ret.2 = true → goal ∈ (has_base_search_state.to_base_state (g:=g) ret.1).visited
+
+abbrev search_returns_with_mother_visited {state_type : Type} [has_base_search_state g state_type]
+    (start : V)
+    (goal : V)
+    (start_to_state : V → state_type)
+    (search_step : search_step_function g)
+    (termination_metric : state_type → ℕ × ℕ)
+    (decreasing_proof : termination_metric_decreasing_proof goal search_step termination_metric):=
+    search_invar_mother_is_visited (has_base_search_state.to_base_state (g:=g) (search_internal start goal start_to_state search_step termination_metric decreasing_proof).1)
+
+abbrev search_returns_with_mother_adjacent {state_type : Type} [has_base_search_state g state_type]
+    (start : V)
+    (goal : V)
+    (start_to_state : V → state_type)
+    (search_step : search_step_function g)
+    (termination_metric : state_type → ℕ × ℕ)
+    (decreasing_proof : termination_metric_decreasing_proof goal search_step termination_metric):=
+    search_invar_mother_is_adjacent start (has_base_search_state.to_base_state (g:=g) (search_internal start goal start_to_state search_step termination_metric decreasing_proof).1)
+
+abbrev search_returns_with_mother_decreasing {state_type : Type} [has_base_search_state g state_type]
+    (start : V)
+    (goal : V)
+    (start_to_state : V → state_type)
+    (search_step : search_step_function g)
+    (termination_metric : state_type → ℕ × ℕ)
+    (decreasing_proof : termination_metric_decreasing_proof goal search_step termination_metric):= 
+    search_invar_mother_decreasing_path_order start (has_base_search_state.to_base_state (g:=g) (search_internal start goal start_to_state search_step termination_metric decreasing_proof).1)
+
+
+def search_exe {state_type : Type} [has_base_search_state g state_type]
+    (start : V)
+    (goal : V)
+    (start_to_state : V → state_type)
+    (search_step : search_step_function g)
+    (termination_metric : state_type → ℕ × ℕ)
+    (decreasing_proof : termination_metric_decreasing_proof goal search_step termination_metric)
+    (goal_if_return_true : search_visited_goal_if_returned_true start goal start_to_state search_step termination_metric decreasing_proof)
+    (mother_visited : search_returns_with_mother_visited start goal start_to_state search_step termination_metric decreasing_proof)
+    (mother_adjacent : search_returns_with_mother_adjacent start goal start_to_state search_step termination_metric decreasing_proof)
+    (mother_decreasing : search_returns_with_mother_decreasing start goal start_to_state search_step termination_metric decreasing_proof):
+    Option (Path g start goal) :=
+  let ret := search_internal start goal start_to_state search_step termination_metric decreasing_proof
+  let final_state:= ret.1
+  let found_goal := ret.2
+
+  if found_goal_true : found_goal = true then
+    some (extract_path_to start goal (has_base_search_state.to_base_state final_state)
+      (goal_if_return_true found_goal_true) mother_visited mother_adjacent mother_decreasing).1
+  else
+    none
+
+theorem search_is_sound {state_type : Type} [has_base_search_state g state_type]
+    (start : V)
+    (goal : V)
+    (start_to_state : V → state_type)
+    (search_step : search_step_function g)
+    (termination_metric : state_type → ℕ × ℕ)
+    (decreasing_proof : termination_metric_decreasing_proof goal search_step termination_metric)
+    (goal_if_return_true : search_visited_goal_if_returned_true start goal start_to_state search_step termination_metric decreasing_proof)
+    (mother_visited : search_returns_with_mother_visited start goal start_to_state search_step termination_metric decreasing_proof)
+    (mother_adjacent : search_returns_with_mother_adjacent start goal start_to_state search_step termination_metric decreasing_proof)
+    (mother_decreasing : search_returns_with_mother_decreasing start goal start_to_state search_step termination_metric decreasing_proof):
+    (Option.isSome (search_exe start goal start_to_state search_step termination_metric decreasing_proof goal_if_return_true mother_visited mother_adjacent mother_decreasing) → (∃ x : (Path g start goal), x = x)) := by
+  intro h -- Option.isSome true on some and false on none, x = x since we need a formula
+  constructor -- since goal is existence
+  rfl
+  let w := Option.get (search_exe start goal start_to_state search_step termination_metric decreasing_proof goal_if_return_true mother_visited mother_adjacent mother_decreasing) -- Option.get extracts value of returned some and fails otherwise
+  apply w
+  simp_all
+
+
+abbrev search_returns_with_start_visited {state_type : Type} [has_base_search_state g state_type]
+    (start : V)
+    (goal : V)
+    (start_to_state : V → state_type)
+    (search_step : search_step_function g)
+    (termination_metric : state_type → ℕ × ℕ)
+    (decreasing_proof : termination_metric_decreasing_proof goal search_step termination_metric):=
+    search_invar_start_visited start (has_base_search_state.to_base_state (g:=g) (search_internal start goal start_to_state search_step termination_metric decreasing_proof).1)
+
+abbrev search_returns_with_node_on_stack_or_all_neighbours_visited {state_type : Type} [has_base_search_state g state_type]
+    (start : V)
+    (goal : V)
+    (start_to_state : V → state_type)
+    (search_step : search_step_function g)
+    (termination_metric : state_type → ℕ × ℕ)
+    (decreasing_proof : termination_metric_decreasing_proof goal search_step termination_metric):=
+    search_invar_on_stack_or_all_neighbours_visited (has_base_search_state.to_base_state (g:=g) (search_internal start goal start_to_state search_step termination_metric decreasing_proof).1)
+
+abbrev search_empty_stack_if_returned_false{state_type : Type} [has_base_search_state g state_type]
+    (start : V)
+    (goal : V)
+    (start_to_state : V → state_type)
+    (search_step : search_step_function g)
+    (termination_metric : state_type → ℕ × ℕ)
+    (decreasing_proof : termination_metric_decreasing_proof goal search_step termination_metric)
+:=
+    (search_internal start goal start_to_state search_step termination_metric decreasing_proof).2 = false → (has_base_search_state.to_base_state (g:=g) (search_internal start goal start_to_state search_step termination_metric decreasing_proof).1).stack = [] 
+
+
+abbrev search_not_visited_goal_if_returned_false{state_type : Type} [has_base_search_state g state_type]
+    (start : V)
+    (goal : V)
+    (start_to_state : V → state_type)
+    (search_step : search_step_function g)
+    (termination_metric : state_type → ℕ × ℕ)
+    (decreasing_proof : termination_metric_decreasing_proof goal search_step termination_metric)
+    :=
+    (search_internal start goal start_to_state search_step termination_metric decreasing_proof).2 = false → goal ∉ (has_base_search_state.to_base_state (g:=g) (search_internal start goal start_to_state search_step termination_metric decreasing_proof).1).visited
+
+
+theorem search_is_complete {state_type : Type} [has_base_search_state g state_type]
+    (start : V)
+    (goal : V)
+    (start_to_state : V → state_type)
+    (search_step : search_step_function g)
+    (termination_metric : state_type → ℕ × ℕ)
+    (decreasing_proof : termination_metric_decreasing_proof goal search_step termination_metric)
+    (goal_if_return_true : search_visited_goal_if_returned_true start goal start_to_state search_step termination_metric decreasing_proof)
+    (mother_visited : search_returns_with_mother_visited start goal start_to_state search_step termination_metric decreasing_proof)
+    (mother_adjacent : search_returns_with_mother_adjacent start goal start_to_state search_step termination_metric decreasing_proof)
+    (mother_decreasing : search_returns_with_mother_decreasing start goal start_to_state search_step termination_metric decreasing_proof)
+    (start_visited : search_returns_with_start_visited start goal start_to_state search_step termination_metric decreasing_proof)
+    (on_stack_or_all_nei_visited : search_returns_with_node_on_stack_or_all_neighbours_visited start goal start_to_state search_step termination_metric decreasing_proof)
+    (stack_empty_if_returned_false : search_empty_stack_if_returned_false start goal start_to_state search_step termination_metric decreasing_proof)
+    (goal_not_visited_if_returned_false : search_not_visited_goal_if_returned_false start goal start_to_state search_step termination_metric decreasing_proof):
+    ((∃ x : (Path g start goal), x = x) → Option.isSome (search_exe start goal start_to_state search_step termination_metric decreasing_proof goal_if_return_true mother_visited mother_adjacent mother_decreasing)) := by
+    -- or Option.isNone (dfs g start goal) → ∄ x (Path g start goal), x = x
+      intro path_exists
+      apply Exists.elim path_exists
+      intro thePath a; clear a-- uninformativ x=X
+
+      let final := search_internal start goal start_to_state search_step termination_metric decreasing_proof
+      let final_state : base_search_state g := has_base_search_state.to_base_state final.1
+      
+      --have start_visited : search_invar_start_visited start final_state :=
+      --  search_returns_with_start_visited start goal start_to_state search_step termination_metric decreasing_proof goal_if_return_true mother_visited mother_adjacent mother_decreasing
+      --have on_stack_or_all_nei_visited : search_invar_on_stack_or_all_neighbours_visited final_state:=
+      --  dfs_returns_with_node_on_stack_or_all_neighbours_visited start goal
+
+
+      by_contra terminates_with_none
+      simp at terminates_with_none
+
+      have dfs_returned_false : (search_internal start goal start_to_state search_step termination_metric decreasing_proof).2 = false := by
+        unfold search_exe at terminates_with_none
+        simp at terminates_with_none
+        exact terminates_with_none
+
+      have final_stack_empty : final_state.stack = [] := stack_empty_if_returned_false dfs_returned_false
+
+      have goal_not_visited : goal ∉ final_state.visited := goal_not_visited_if_returned_false dfs_returned_false
+
+      obtain ⟨theWalk, nodupe ⟩ := thePath
+      have goal_in_final := search_termination_with_empty_stack_implies_goal_visited start goal start theWalk final_state start_visited final_stack_empty on_stack_or_all_nei_visited
+      contradiction
+
+
+theorem search_is_complete_inv  {state_type : Type} [has_base_search_state g state_type]
+    (start : V)
+    (goal : V)
+    (start_to_state : V → state_type)
+    (search_step : search_step_function g)
+    (termination_metric : state_type → ℕ × ℕ)
+    (decreasing_proof : termination_metric_decreasing_proof goal search_step termination_metric)
+    (goal_if_return_true : search_visited_goal_if_returned_true start goal start_to_state search_step termination_metric decreasing_proof)
+    (mother_visited : search_returns_with_mother_visited start goal start_to_state search_step termination_metric decreasing_proof)
+    (mother_adjacent : search_returns_with_mother_adjacent start goal start_to_state search_step termination_metric decreasing_proof)
+    (mother_decreasing : search_returns_with_mother_decreasing start goal start_to_state search_step termination_metric decreasing_proof)
+    (start_visited : search_returns_with_start_visited start goal start_to_state search_step termination_metric decreasing_proof)
+    (on_stack_or_all_nei_visited : search_returns_with_node_on_stack_or_all_neighbours_visited start goal start_to_state search_step termination_metric decreasing_proof)
+    (stack_empty_if_returned_false : search_empty_stack_if_returned_false start goal start_to_state search_step termination_metric decreasing_proof)
+    (goal_not_visited_if_returned_false : search_not_visited_goal_if_returned_false start goal start_to_state search_step termination_metric decreasing_proof):
+    Option.isNone (search_exe start goal start_to_state search_step termination_metric decreasing_proof goal_if_return_true mother_visited mother_adjacent mother_decreasing) → ¬ ∃ x : (Path g start goal), x = x := by
+      intro optionIsNone
+      by_contra pathExists
+      have isSome := search_is_complete start goal start_to_state search_step termination_metric decreasing_proof goal_if_return_true mother_visited mother_adjacent mother_decreasing start_visited on_stack_or_all_nei_visited stack_empty_if_returned_false goal_not_visited_if_returned_false
+      simp_all
